concur/CMulti.v
@@ -50,7 +50,7 @@ Module NatMap := IRMap(NatIndexed).
     Now this two points are implemented differernt with CASCompCert *)
 Section MultiThread.
 
-  Context {OpenS : semantics li_c li_c}.
+  Variable OpenS : semantics li_c li_c.
 
   Definition local_state := state OpenS.
 
@@ -61,11 +61,13 @@ Section MultiThread.
 
   Definition get_cqv (q: c_query) :=
     cqv (cq_vf q) (cq_sg q) (cq_args q).
-  
-  Definition thread_state :Type := local_state + cq_vals.
+
+  Inductive thread_state : Type :=
+  |Local : forall (ls : local_state), thread_state
+  |Initial : forall (cqv : cq_vals), thread_state
+  |Return : forall (ls : local_state), thread_state.
   
   Definition initial_se := Genv.symboltbl (skel OpenS).
-  (* Variable initial_se : Genv.symtbl. *)
   
   Definition OpenLTS := activate OpenS initial_se.
   
@@ -109,9 +111,20 @@ Section MultiThread.
 
   Definition update_next_tid (s: state) (tid: nat) :=
     mk_gstate (threads s) (cur_tid s) tid.
+
+  Fixpoint yield_strategy' (threads: NatMap.t (option thread_state)) (next: nat) :=
+    match next with
+    |O | S O => 1%nat (*next should be >= 2, this is meaningless*)
+    |S n => (* n is the max valid thread id*)
+       match NatMap.get n threads with
+       | Some (Initial _) | Some (Return _) => n
+       | _ => yield_strategy' threads n
+       end
+    end.
   
-  Variable yield_strategy : state -> nat.
-  Axiom yield_strategy_range : forall s, (1 < yield_strategy s < (next_tid s))%nat.
+  Definition yield_strategy (s:state) := yield_strategy' (threads s) (next_tid s).
+  
+  (* Axiom yield_strategy_range : forall s, (1 < yield_strategy s < (next_tid s))%nat. *)
   (*some other properties may be added here, such as only point to active threads *)
 
   (* We transfer to thread tid' and update
@@ -127,16 +140,12 @@ Section MultiThread.
   Definition pthread_create_state (s: state) (cqv : cq_vals) (ls' : thread_state): state :=
     let ntid := (next_tid s) in let ctid := (cur_tid s) in
     let s' := update_next_tid s (S ntid) in
-    let s'' := update_thread s' ntid (inr cqv) in
+    let s'' := update_thread s' ntid (Initial cqv) in
     update_thread s'' ctid ls'.
     
   Definition genvtype := Smallstep.genvtype OpenLTS.
   
   (** Initial state of Concurrent semantics *)
-
-  (*Variable initial_query : query li_c.
-    Variable final_reply : int -> reply li_c -> Prop. *)
-  (* Definition ClosedS := Closed.close_semantics initial_query final_reply OpenS initial_se. *)
 
   (** Construct the initial memory *)
   Definition main_id := prog_main (skel OpenS).
@@ -145,7 +154,7 @@ Section MultiThread.
   Inductive initial_state : state -> Prop :=
   |initial_state_intro : forall ls s main_b m0,
       cur_tid s = 1%nat -> next_tid s = 2%nat ->
-      get_cur_thread s = Some (inl ls) ->
+      get_cur_thread s = Some (Local ls) ->
       Genv.find_symbol initial_se main_id = Some main_b ->
       Genv.init_mem (skel OpenS) = Some m0 ->
       (Smallstep.initial_state OpenLTS)
@@ -157,7 +166,7 @@ Section MultiThread.
   Inductive final_state : state -> int -> Prop :=  
   |final_state_intro : forall ls i s m,
       cur_tid s = 1%nat ->
-      get_cur_thread s = Some (inl ls) ->
+      get_cur_thread s = Some (Local ls) ->
       (Smallstep.final_state OpenLTS) ls (cr (Vint i) m)->
       final_state s i.
 
@@ -200,42 +209,42 @@ Section MultiThread.
   
   Inductive step : genvtype -> state -> trace -> state -> Prop :=
   |step_local : forall ge ls1 t ls2 s s',
-      get_cur_thread s = Some (inl ls1) ->
+      get_cur_thread s = Some (Local ls1) ->
       Smallstep.step OpenLTS ge ls1 t ls2 ->
-      update_thread s (cur_tid s) (inl ls2) = s' ->
+      update_thread s (cur_tid s) (Local ls2) = s' ->
       step ge s t s'
   |step_thread_create : forall ge s s' q_ptc q_str gmem ls ls' cqv,
-      get_cur_thread s = Some (inl ls) -> (* get the current local state *)
+      get_cur_thread s = Some (Local ls) -> (* get the current local state *)
       Smallstep.at_external OpenLTS ls q_ptc -> (* get the query to pthread_create *)
       query_is_pthread_create q_ptc q_str -> (* get the query to start_routine *)
       (* The global memory is already updated from q_ptc to q_str *)
       cq_mem q_str = gmem -> (* the updated memory, only difference is the #threads *)
       get_cqv q_str = cqv -> (*the initial query without memory, is stored as initial state in new thread *)
       Smallstep.after_external OpenLTS ls (cr (Vint Int.one) gmem) ls' -> (* the current thread completes the primitive*)
-      pthread_create_state s cqv (inl ls') = s' ->
+      pthread_create_state s cqv (Local ls') = s' ->
       step ge s E0 s'
   (** yield to a thread which is waiting for the reply of its own [yield()] *)
   |step_thread_yield_to_yield : forall ge s s' tid' q gmem' p ls ls1 ls1',
-      get_cur_thread s = Some (inl ls) ->
+      get_cur_thread s = Some (Local ls) ->
       Smallstep.at_external OpenLTS ls q ->
       query_is_yield q ->
       yield_strategy s = tid' ->
       (*the proof p may be a problem, provided from the invariant between state and the support in gmem *)
       Mem.yield (cq_mem q) tid' p = gmem' ->
-      get_thread s (tid') = Some (inl ls1) -> (* the target thread is waiting for reply *)
+      get_thread s (tid') = Some (Return ls1) -> (* the target thread is waiting for reply *)
       Smallstep.after_external OpenLTS ls1 (cr Vundef gmem') ls1' ->
-      yield_state s (inl ls1') = s' ->
+      yield_state s (Local ls1') = s' ->
       step ge s E0 s'
   (** yield to a thread which has not been initialized from a query *)
   |step_thread_yield_to_initial : forall ge s s' tid' q gmem' p ls cqv ls1',
-      get_cur_thread s = Some (inl ls) ->
+      get_cur_thread s = Some (Local ls) ->
       Smallstep.at_external OpenLTS ls q ->
       query_is_yield q ->
       yield_strategy s = tid' ->
       Mem.yield (cq_mem q) tid' p = gmem' ->
-      get_thread s (tid') = Some (inr cqv) -> (* the target thread is waiting for reply *)
+      get_thread s (tid') = Some (Initial cqv) -> (* the target thread is waiting for reply *)
       Smallstep.initial_state OpenLTS (get_query cqv gmem') ls1' ->
-      yield_state s (inl ls1') = s' ->
+      yield_state s (Local ls1') = s' ->
       step ge s E0 s'.
 
   Definition globalenv := Smallstep.globalenv OpenLTS.
